coqimp/contextswitch/proof/WindowOKProof.v
@@ -1,5 +1,5 @@
-Require Import Coqlib.                          
-Require Import Maps.           
+Require Import Coqlib.                                
+Require Import Maps.            
 Require Import LibTactics.   
         
 Require Import Integers.  
@@ -51,6 +51,44 @@ Proof.
     destruct (zeq (Int.unsigned $ 84) (Int.unsigned $ 4095)) eqn:Heqe3; eauto; tryfalse.
 Qed.
 
+(*+ Lemmas for Space +*)
+Lemma getR_eq_get_genreg_val1 :
+  forall M R F D grst (rr : GenReg) p,
+    (M, (R, F), D) |= GenRegs grst ** p ->
+    get_R R rr = Some (get_genreg_val grst rr).
+Proof.
+  intros.
+  sep_star_split_tac.
+  simpl in H3.
+  simpljoin1.
+  eapply get_R_merge_still; eauto.
+  eapply getR_eq_get_genreg_val; eauto.
+Qed.
+
+(*+ Lemmas for Inference Rule +*)
+Theorem getcwp_rule_reg_fm :
+  forall grst rd p id vi F,
+    |- {{ GenRegs grst ** FrameState id vi F ** p }}
+        getcwp rd
+      {{ GenRegs (upd_genreg grst rd id) ** FrameState id vi F ** p }}.
+Proof.
+  intros.
+  eapply ins_conseq_rule.
+  introv Hs.
+  simpl_sep_liftn_in Hs 2.
+  unfold FrameState in Hs.
+  asrt_to_line_in Hs 3.
+  simpl_sep_liftn_in Hs 5.
+  eauto.
+  eapply getcwp_rule_reg; eauto.
+  introv Hs.
+  sep_cancel1 1 1.
+  unfold FrameState.
+  asrt_to_line 3.
+  eauto.
+Qed.
+
+(*+ Proof +*)
 Theorem Ta0WindowOKProof :
   forall vl,
     spec |- {{ ta0_window_ok_pre vl }}
@@ -180,6 +218,155 @@ Proof.
   unfold OS_CONTEXT_OFFSET.
   rewrite in_range84; eauto.
   simpl upd_genreg.
+ 
+  (** call reg_save; nop *)
+  clear Hlgvl.
+  eapply call_rule.
+  {
+    eval_spec.
+  }
+  {
+    introv Hs.
+    TimReduce_simpl_in Hs.
+    eapply GenRegs_split_one with (rr := r15) in Hs.
+    simpls get_genreg_val'.
+    eauto.
+  }
+  {
+    TimReduce_simpl.
+    eapply nop_rule; eauto.
+  }
+  {   
+    unfold reg_save_pre.
+    instantiate (1 :=
+                   logic_fm ([[ct -ᵢ ($ 0), w0, w1, w2, w3, w4, w5, w6]])
+                            :: logic_fm ([[w7, w8, w9, w10, w11, w12, w13, $ 204]])
+                            :: logic_fm ([[w15, w16, w17, w18, ct, ct +ᵢ ($ 84), w21, w22]])
+                            :: logic_fm ([[w23, w24, w25, w26, w27, w28, w29, w30]])
+                            :: logic_lv id :: logic_lv vi :: logic_fmls F
+                            :: logic_lv vy :: logic_lv ($ 204) :: nil).
+    introv Hs. 
+    sep_ex_elim_in Hs.
+    eapply sep_pure_l_elim in Hs.
+    destruct Hs as [Hlgvl_save Hs].
+    symmetry in Hlgvl_save.
+    inversion Hlgvl_save; subst.
+    clear Hlgvl_save.
+    simpl_sep_liftn_in Hs 5.
+    eapply sep_pure_l_elim in Hs.
+    destruct Hs as [Hpure Hs].
+    simpljoin1.
+    match goal with
+    | H : get_frame_nth _ 7 = Some _ |- _ =>
+      renames H to Hretf
+    end.
+    simpl in Hretf.
+    inversion Hretf; subst.
+    simpl.
+    destruct_state s.
+    simpl.
+    clear - Hs. 
+    eapply getR_eq_get_genreg_val1 with (rr := r15) in Hs; eauto.
+  }
+  {
+    introv Hs.
+    eapply GenRegs_upd_combine_one in Hs.
+    simpl upd_genreg in Hs.
+    unfold reg_save_pre.
+    sep_ex_intro.
+    asrt_to_line 5.
+    eapply sep_pure_l_intro; eauto.  
+    sep_cancel1 1 1.
+    sep_cancel1 9 1.
+    sep_cancel1 6 1.
+    sep_cancel1 5 1.
+    simpl get_frame_nth.
+    eapply sep_pure_l_intro; eauto.
+  }
+  {
+    eauto.
+  }
+  {  
+    unfold reg_save_post.
+    introv Hs.
+    sep_ex_elim_in Hs.
+    eapply sep_pure_l_elim in Hs.
+    destruct Hs as [Hlgvl1 Hs].
+    symmetry in Hlgvl1.
+    inversion Hlgvl1; subst.
+    clear Hlgvl1.
+    simpl.
+    destruct_state s.
+    simpl.
+    simpl_sep_liftn_in Hs 5.
+    eapply sep_pure_l_elim in Hs.
+    destruct Hs as [Hpure Hs].
+    simpljoin1.
+    match goal with
+    | H : get_frame_nth _ 7 = Some _ |- _ => renames H to Hretf
+    end.
+    simpl in Hretf.
+    inversion Hretf; subst.
+    eapply getR_eq_get_genreg_val1 with (rr := r15) in Hs; eauto.
+  }
+  {
+    DlyFrameFree_elim.
+  }
 
+  unfold reg_save_post.
+  hoare_ex_intro_pre.
+  eapply backward_rule.
+  introv Hs.
+  asrt_to_line_in Hs 5.
+  eauto.
+  eapply Pure_intro_rule.
+  introv Hlgvl.
+  symmetry in Hlgvl.
+  inversion Hlgvl; subst.
+  clear Hlgvl.
+  renames x'3 to cctx'.
+
+  (** getcwp g4 *) 
+  hoare_lift_pre 4.
+  hoare_lift_pre 2.
+  eapply seq_rule.
+  TimReduce_simpl.
+  eapply getcwp_rule_reg_fm; eauto.
+  simpl upd_genreg. 
+
+  (** rd wim g7 *)
+  eapply seq_rule.
+  TimReduce_simpl.
+  eapply rd_rule_reg_wim; eauto.
+  simpl upd_genreg.
+
+  (** set 1 g6 *)
+  eapply seq_rule.
+  TimReduce_simpl.
+  eapply set_rule_reg; eauto.
+  simpl upd_genreg.
+
+  (** sll g6 g4 g4 *)
+  eapply seq_rule.
+  TimReduce_simpl.
+  eapply sll_rule_reg; eauto.
+  simpl upd_genreg.
+  simpl in Hpt_ctx. 
+  inversion Hpt_ctx; subst.
+  eapply hoare_pure_gen' with (pu := $ 0 <=ᵤᵢ id <=ᵤᵢ $ 7 /\ $ 0 <=ᵤᵢ vi <=ᵤᵢ $ 7).
+  {
+    introv Hs.
+    simpl_sep_liftn_in Hs 2.
+    unfold FrameState in Hs.
+    asrt_to_line_in Hs 3.
+    simpl_sep_liftn_in Hs 4.
+    eapply sep_pure_l_elim in Hs.
+    simpljoin1; eauto.
+  }
+  eapply Pure_intro_rule.
+  introv Hin_range.
+  destruct Hin_range as [Hid_inrange Hvi_inrange].
+  rewrite get_range_0_4_stable; eauto.
+  
 Admitted.
   
